open import Data.Nat             using (â„•; zero; suc; _â‰¤_; zâ‰¤n; sâ‰¤s; _<_)
open import Data.Product --        using (Î£; _,_; projâ‚; projâ‚‚; Î£-syntax)
open import Data.Sum             using (_âŠŽ_; injâ‚; injâ‚‚;  [_,_] )
open import Data.Empty          -- using (âŠ¥; âŠ¥-elim)
open import Data.Unit            using (âŠ¤; tt)
-- open import Relation.Binary.PropositionalEquality using (_â‰¡_; refl; sym; cong; subst)
-- open import Data.List            using (List; []; _âˆ·_; _++_; length; map)
open import Data.List.Properties using (map-id; map-compose)
open import Function using (id; _âˆ˜_)
import Relation.Binary.PropositionalEquality as Eq
open Eq                          using (_â‰¡_; refl; sym; trans; cong; subst)
open Eq.â‰¡-Reasoning              using (begin_; _â‰¡âŸ¨âŸ©_; step-â‰¡; _âˆŽ)

import STLC
open import Signature

module Interpreter (ð•Š : Signature.Signature) where

open STLC ð•Š
open Signature.Signature ð•Š
 
data Tree (P : â„‚ â†’ Set) (A : â„‚ â†’ Set) : Set where
  Constr   : âˆ€(c : â„‚)
           â†’ P c
           â†’ (A c â†’ Tree P A)
           --------------------
           â†’ Tree P A

Fold     : {P : â„‚ â†’ Set} {A : â„‚ â†’ Set} {B : Set}
           â†’ (âˆ€ (c : â„‚) â†’ P c â†’ (A c â†’ B) â†’ B)
           â†’ Tree P A
           --------------------
           â†’ B

Fold f (Constr c p t) = f c p (Fold f âˆ˜ t)

âŸ¦_âŸ§áµ : Ground BaseType â†’ Set
âŸ¦ baseáµ b âŸ§áµ = I b
âŸ¦ emptyáµ âŸ§áµ = âŠ¥
âŸ¦ unitáµ âŸ§áµ = âŠ¤
âŸ¦ A +áµ B âŸ§áµ = âŸ¦ A âŸ§áµ âŠŽ âŸ¦ B âŸ§áµ
âŸ¦ A Ã—áµ B âŸ§áµ = âŸ¦ A âŸ§áµ Ã— âŸ¦ B âŸ§áµ

postulate K : âˆ€ (c : Const) â†’ âŸ¦ ConstArg c âŸ§áµ â†’ âŸ¦ ConstResult c âŸ§áµ 

âŸ¦_âŸ§ : Type â†’ Set
âŸ¦ base b âŸ§ = I b
âŸ¦ unit âŸ§ = âŠ¤
âŸ¦ empty âŸ§ = âŠ¥
âŸ¦ A Ã—áµ— B âŸ§ = âŸ¦ A âŸ§ Ã— âŸ¦ B âŸ§
âŸ¦ A â‡’áµ— B âŸ§ = âŸ¦ A âŸ§ â†’ âŸ¦ B âŸ§
âŸ¦ A +áµ— B âŸ§ = âŸ¦ A âŸ§ âŠŽ âŸ¦ B âŸ§
âŸ¦ tree âŸ§ = Tree (Î» c â†’ âŸ¦ par c âŸ§áµ) (Î» c â†’ âŸ¦ ar c âŸ§áµ)  -- termination checking failed

âŸ¦âŸ§áµâ‰¡âŸ¦JâŸ§ : (A : Ground BaseType) â†’ âŸ¦ A âŸ§áµ â‰¡ âŸ¦ J A âŸ§
âŸ¦âŸ§áµâ‰¡âŸ¦JâŸ§ (baseáµ b) = refl
âŸ¦âŸ§áµâ‰¡âŸ¦JâŸ§ emptyáµ = refl
âŸ¦âŸ§áµâ‰¡âŸ¦JâŸ§ unitáµ = refl
âŸ¦âŸ§áµâ‰¡âŸ¦JâŸ§ (A +áµ B) = 
  begin
    (âŸ¦ A âŸ§áµ âŠŽ âŸ¦ B âŸ§áµ)  â‰¡âŸ¨ cong (âŸ¦ A âŸ§áµ âŠŽ_) (âŸ¦âŸ§áµâ‰¡âŸ¦JâŸ§ B) âŸ©
    (âŸ¦ A âŸ§áµ âŠŽ âŸ¦ J B âŸ§)  â‰¡âŸ¨ cong (_âŠŽ âŸ¦ J B âŸ§) (âŸ¦âŸ§áµâ‰¡âŸ¦JâŸ§ A) âŸ©
    (âŸ¦ J A âŸ§ âŠŽ âŸ¦ J B âŸ§)
  âˆŽ
âŸ¦âŸ§áµâ‰¡âŸ¦JâŸ§ (A Ã—áµ B) = 
  begin
    (âŸ¦ A âŸ§áµ Ã— âŸ¦ B âŸ§áµ)  â‰¡âŸ¨ cong (âŸ¦ A âŸ§áµ Ã—_) (âŸ¦âŸ§áµâ‰¡âŸ¦JâŸ§ B) âŸ©
    (âŸ¦ A âŸ§áµ Ã— âŸ¦ J B âŸ§)  â‰¡âŸ¨ cong (_Ã— âŸ¦ J B âŸ§) (âŸ¦âŸ§áµâ‰¡âŸ¦JâŸ§ A) âŸ©
    (âŸ¦ J A âŸ§ Ã— âŸ¦ J B âŸ§)
  âˆŽ

âŸ¦_âŸ§â‚‘ : Ctx â†’ Set
âŸ¦ [] âŸ§â‚‘ = âŠ¤ -- âŠ¥
âŸ¦ Î“ âˆ· A âŸ§â‚‘ = âŸ¦ Î“ âŸ§â‚‘ Ã— âŸ¦ A âŸ§


aux-proj : {A : Type} {Î“ : Ctx} â†’ A âˆˆ Î“ â†’ âŸ¦ Î“ âŸ§â‚‘ â†’ âŸ¦ A âŸ§
aux-proj âˆˆ-here (_ , x) = x
aux-proj (âˆˆ-there index) (xs , _) = aux-proj index xs

lemica : {A B : Set} â†’ A â‰¡ B â†’ A â†’ B
lemica refl p = p

âŸ¦_âŸ§áµ¢ : {Î“ : Ctx} {A : Type} â†’ Î“ âŠ¢ A â†’ (âŸ¦ Î“ âŸ§â‚‘ â†’ âŸ¦ A âŸ§)
âŸ¦ var index âŸ§áµ¢ Î· = aux-proj index Î·
âŸ¦ const c args âŸ§áµ¢ Î· =  lemica (âŸ¦âŸ§áµâ‰¡âŸ¦JâŸ§ (ConstResult c)) (K c (lemica (sym (âŸ¦âŸ§áµâ‰¡âŸ¦JâŸ§ (ConstArg c))) (âŸ¦ args âŸ§áµ¢ Î·))) --  {! K c (âŸ¦ args âŸ§áµ¢ Î·)  !}
âŸ¦ unit âŸ§áµ¢ _  = tt
âŸ¦ absurd t âŸ§áµ¢ =  âŠ¥-elim âˆ˜ âŸ¦ t âŸ§áµ¢
âŸ¦ t Ø› u âŸ§áµ¢ Î· =  âŸ¦ t âŸ§áµ¢  Î· , âŸ¦ u âŸ§áµ¢  Î·
âŸ¦ fst t âŸ§áµ¢ Î· = projâ‚ (âŸ¦ t âŸ§áµ¢  Î·)
âŸ¦ snd t âŸ§áµ¢ Î· = projâ‚‚ (âŸ¦ t âŸ§áµ¢  Î·)
âŸ¦ inl t âŸ§áµ¢ Î· = injâ‚ (âŸ¦ t âŸ§áµ¢  Î·)
âŸ¦ inr t âŸ§áµ¢ Î· = injâ‚‚ (âŸ¦ t âŸ§áµ¢  Î·)
âŸ¦ case t uâ‚ uâ‚‚ âŸ§áµ¢ Î· = [ ( Î» z â†’ âŸ¦  uâ‚ âŸ§áµ¢ ( Î· , z) ) , (( Î» z â†’ âŸ¦  uâ‚‚ âŸ§áµ¢ ( Î· , z) )) ] ((âŸ¦ t âŸ§áµ¢  Î·))
âŸ¦ fun t âŸ§áµ¢ Î· = Î» z â†’ âŸ¦ t âŸ§áµ¢ (Î· , z)
âŸ¦ app t u âŸ§áµ¢ Î· = (âŸ¦ t âŸ§áµ¢  Î·) (âŸ¦ u âŸ§áµ¢  Î·)
âŸ¦ constr c param args âŸ§áµ¢ Î· =  Constr c (lemica (sym (âŸ¦âŸ§áµâ‰¡âŸ¦JâŸ§ (par c))) (âŸ¦ param âŸ§áµ¢ Î·)) Î» i â†’ âŸ¦ args âŸ§áµ¢ (Î· , lemica (âŸ¦âŸ§áµâ‰¡âŸ¦JâŸ§ (ar c)) i)
âŸ¦ fold f t âŸ§áµ¢ Î· = Fold (Î» c p t' â†’ âŸ¦ f c âŸ§áµ¢ ((Î· , lemica (âŸ¦âŸ§áµâ‰¡âŸ¦JâŸ§ (par c)) p) , Î» x â†’ t' (lemica (sym (âŸ¦âŸ§áµâ‰¡âŸ¦JâŸ§ (ar c))) x)) ) (âŸ¦ t âŸ§áµ¢ Î·)
